examples/ml_example/output.dfy
@@ -1,189 +1,193 @@
-function Ls(s: seq2D): (seq<int>)
+function Ls(s: seq2D): seq<int>
     ensures |Ls(s)| == width(s)
 {
-    var LsRes := (if s == [] then [] else if |s| == 1 then preSum(s[0]) else vAdd(Ls(s[..|s|-1]), preSum(s[|s|-1])));
+    var LsRes := if s == [] then [] else if |s| == 1 then preSum(s[0]) else vAdd(Ls(s[..|s|-1]), preSum(s[|s|-1]));
     (LsRes)
 }
 
-function Mbl(s: seq2D): ((seq<int>), (seq<int>))
+function Mbl(s: seq2D): (seq<int>, seq<int>)
     decreases |s|
     ensures |Mbl(s).0| == width(s)
 {
-    var MblRes := (if s == [] then [] else if |s| == 1 then pMax(preSum(s[0]), zeroSeq(|s[0]|))
-        else pMax(Mbl([s[|s|-1]]).0, vAdd(Mbl(s[..|s|-1]).0, preSum(s[|s|-1]))));
+    var MblRes := if s == [] then [] else if |s| == 1 then pMax(preSum(s[0]), zeroSeq(|s[0]|))
+        else pMax(Mbl([s[|s|-1]]).0, vAdd(Mbl(s[..|s|-1]).0, preSum(s[|s|-1])));
     var LsRes := Ls(s);
     (MblRes, LsRes)
 }
 
-function Mtl(s: seq2D): ((seq<int>), (seq<int>))
+function Mtl(s: seq2D): (seq<int>, seq<int>)
     decreases |s|
     ensures |Mtl(s).0| == width(s)
 {
-    var MtlRes := (if s == [] then [] else if |s| == 1 then pMax(preSum(s[0]), zeroSeq(|s[0]|))
-        else pMax(Mtl(s[..|s|-1]).0, vAdd(Mtl([s[|s|-1]]).0, Ls(s[..|s|-1]))));
+    var MtlRes := if s == [] then [] else if |s| == 1 then pMax(preSum(s[0]), zeroSeq(|s[0]|))
+        else pMax(Mtl(s[..|s|-1]).0, vAdd(Mtl([s[|s|-1]]).0, Ls(s[..|s|-1])));
     var LsRes := Ls(s);
     (MtlRes, LsRes)
 }
 
-function Ml(s: seq2D): ((seq<int>), ((seq<int>), (seq<int>)), ((seq<int>), (seq<int>)))
+function Ml(s: seq2D): (seq<int>, (seq<int>, seq<int>), (seq<int>, seq<int>))
     decreases |s|
     ensures |Ml(s).0| == width(s)
 {
-    var MlRes := (if s == [] then [] else if |s| == 1 then pMax(preSum(s[0]), zeroSeq(|s[0]|))
-                                else pMax(pMax(Ml(s[..|s|-1]).0, Ml([s[|s|-1]]).0), vAdd(Mbl(s[..|s|-1]).0, Mtl([s[|s|-1]]).0)));
+    var MlRes := if s == [] then [] else if |s| == 1 then pMax(preSum(s[0]), zeroSeq(|s[0]|))
+        else pMax(pMax(Ml(s[..|s|-1]).0, Ml([s[|s|-1]]).0), vAdd(Mbl(s[..|s|-1]).0, Mtl([s[|s|-1]]).0));
     var MblRes := Mbl(s);
     var MtlRes := Mtl(s);
     (MlRes, MblRes, MtlRes)
 }
 
-function LsJoin(a: (seq<int>), b: (seq<int>)): (seq<int>)
+function LsJoin(a: seq<int>, b: seq<int>): seq<int>
     requires |a| == |b|
 {
-    var LsRes := (vAdd(a, b));
+    var LsRes := vAdd(a, b);
     (LsRes)
 }
 
-function MblJoin(a: ((seq<int>), (seq<int>)), b: ((seq<int>), (seq<int>))): ((seq<int>), (seq<int>))
+function MblJoin(a: (seq<int>, seq<int>), b: (seq<int>, seq<int>)): (seq<int>, seq<int>)
     requires |a.0| == |a.1| == |b.0| == |b.1|
 {
-    var MblRes := (pMax(b.0, vAdd(a.0, b.1)));
+    var MblRes := pMax(b.0, vAdd(a.0, b.1));
     var LsRes := LsJoin(a.1, b.1);
     (MblRes, LsRes)
 }
 
-function MtlJoin(a: ((seq<int>), (seq<int>)), b: ((seq<int>), (seq<int>))): ((seq<int>), (seq<int>))
+function MtlJoin(a: (seq<int>, seq<int>), b: (seq<int>, seq<int>)): (seq<int>, seq<int>)
     requires |a.0| == |a.1| == |b.0| == |b.1|
 {
-    var MtlRes := (pMax(a.0, vAdd(b.0, a.1)));
+    var MtlRes := pMax(a.0, vAdd(b.0, a.1));
     var LsRes := LsJoin(a.1, b.1);
     (MtlRes, LsRes)
 }
 
-function MlJoin(a: ((seq<int>), ((seq<int>), (seq<int>)), ((seq<int>), (seq<int>))), b: ((seq<int>), ((seq<int>), (seq<int>)), ((seq<int>), (seq<int>)))): ((seq<int>), ((seq<int>), (seq<int>)), ((seq<int>), (seq<int>)))
+function MlJoin(a: (seq<int>, (seq<int>, seq<int>), (seq<int>, seq<int>)), b: (seq<int>, (seq<int>, seq<int>), (seq<int>, seq<int>))): (seq<int>, (seq<int>, seq<int>), (seq<int>, seq<int>))
     requires |a.0| == |a.1.0| == |a.1.1| == |a.2.0| == |a.2.1| == |b.0| == |b.1.0| == |b.1.1| == |b.2.0| == |b.2.1|
 {
-    var MlRes := (pMax(pMax(a.0, b.0), vAdd(a.1.0, b.2.0)));
+    var MlRes := pMax(pMax(a.0, b.0), vAdd(a.1.0, b.2.0));
     var MblRes := MblJoin(a.1, b.1);
     var MtlRes := MtlJoin(a.2, b.2);
     (MlRes, MblRes, MtlRes)
 }
 
-lemma LsJoinAssoc(a: (seq<int>), b: (seq<int>), c: (seq<int>))
+lemma LsJoinAssoc(a: seq<int>, b: seq<int>, c: seq<int>)
     decreases |a|, |b|, |c|
     requires |a| == |b| == |c| 
     ensures LsJoin(LsJoin(a, b), c) == LsJoin(a, LsJoin(b, c))
 {
-    if |a| == 0 {}
-    else if |a| == 1 {}
+    var n := |a|;
+    if n == 0 {}
+    else if n == 1 {}
     else
     {
-        var a' := a[..|a|-1];
-        var b' := b[..|b|-1];
-        var c' := c[..|c|-1];
+        var a' := a[..n-1];
+        var b' := b[..n-1];
+        var c' := c[..n-1];
         LsJoinAssoc((a'), (b'), (c'));
 
-        var af := [a[|a|-1]];
-        var bf := [b[|b|-1]];
-        var cf := [c[|c|-1]];
+        var af := [a[n-1]];
+        var bf := [b[n-1]];
+        var cf := [c[n-1]];
         LsJoinAssoc((af), (bf), (cf));
     }
 }
 
-lemma MblJoinAssoc(a: ((seq<int>), (seq<int>)), b: ((seq<int>), (seq<int>)), c: ((seq<int>), (seq<int>)))
+lemma MblJoinAssoc(a: (seq<int>, seq<int>), b: (seq<int>, seq<int>), c: (seq<int>, seq<int>))
     decreases |a.0|, |a.1|, |b.0|, |b.1|, |c.0|, |c.1|
     requires |a.0| == |a.1| == |b.0| == |b.1| == |c.0| == |c.1| 
     ensures MblJoin(MblJoin(a, b), c) == MblJoin(a, MblJoin(b, c))
 {
-    if |a.0| == 0 {}
-    else if |a.0| == 1 {}
+    var n := |a.0|;
+    if n == 0 {}
+    else if n == 1 {}
     else
     {
-        var a0' := a.0[..|a.0|-1];
-        var a1' := a.1[..|a.1|-1];
-        var b0' := b.0[..|b.0|-1];
-        var b1' := b.1[..|b.1|-1];
-        var c0' := c.0[..|c.0|-1];
-        var c1' := c.1[..|c.1|-1];
+        var a0' := a.0[..n-1];
+        var a1' := a.1[..n-1];
+        var b0' := b.0[..n-1];
+        var b1' := b.1[..n-1];
+        var c0' := c.0[..n-1];
+        var c1' := c.1[..n-1];
         MblJoinAssoc(((a0', a1')), ((b0', b1')), ((c0', c1')));
 
-        var a0f := [a.0[|a.0|-1]];
-        var a1f := [a.1[|a.1|-1]];
-        var b0f := [b.0[|b.0|-1]];
-        var b1f := [b.1[|b.1|-1]];
-        var c0f := [c.0[|c.0|-1]];
-        var c1f := [c.1[|c.1|-1]];
+        var a0f := [a.0[n-1]];
+        var a1f := [a.1[n-1]];
+        var b0f := [b.0[n-1]];
+        var b1f := [b.1[n-1]];
+        var c0f := [c.0[n-1]];
+        var c1f := [c.1[n-1]];
         MblJoinAssoc(((a0f, a1f)), ((b0f, b1f)), ((c0f, c1f)));
     }
 }
 
-lemma MtlJoinAssoc(a: ((seq<int>), (seq<int>)), b: ((seq<int>), (seq<int>)), c: ((seq<int>), (seq<int>)))
+lemma MtlJoinAssoc(a: (seq<int>, seq<int>), b: (seq<int>, seq<int>), c: (seq<int>, seq<int>))
     decreases |a.0|, |a.1|, |b.0|, |b.1|, |c.0|, |c.1|
     requires |a.0| == |a.1| == |b.0| == |b.1| == |c.0| == |c.1| 
     ensures MtlJoin(MtlJoin(a, b), c) == MtlJoin(a, MtlJoin(b, c))
 {
-    if |a.0| == 0 {}
-    else if |a.0| == 1 {}
+    var n := |a.0|;
+    if n == 0 {}
+    else if n == 1 {}
     else
     {
-        var a0' := a.0[..|a.0|-1];
-        var a1' := a.1[..|a.1|-1];
-        var b0' := b.0[..|b.0|-1];
-        var b1' := b.1[..|b.1|-1];
-        var c0' := c.0[..|c.0|-1];
-        var c1' := c.1[..|c.1|-1];
+        var a0' := a.0[..n-1];
+        var a1' := a.1[..n-1];
+        var b0' := b.0[..n-1];
+        var b1' := b.1[..n-1];
+        var c0' := c.0[..n-1];
+        var c1' := c.1[..n-1];
         MtlJoinAssoc(((a0', a1')), ((b0', b1')), ((c0', c1')));
 
-        var a0f := [a.0[|a.0|-1]];
-        var a1f := [a.1[|a.1|-1]];
-        var b0f := [b.0[|b.0|-1]];
-        var b1f := [b.1[|b.1|-1]];
-        var c0f := [c.0[|c.0|-1]];
-        var c1f := [c.1[|c.1|-1]];
+        var a0f := [a.0[n-1]];
+        var a1f := [a.1[n-1]];
+        var b0f := [b.0[n-1]];
+        var b1f := [b.1[n-1]];
+        var c0f := [c.0[n-1]];
+        var c1f := [c.1[n-1]];
         MtlJoinAssoc(((a0f, a1f)), ((b0f, b1f)), ((c0f, c1f)));
     }
 }
 
-lemma MlJoinAssoc(a: ((seq<int>), ((seq<int>), (seq<int>)), ((seq<int>), (seq<int>))), b: ((seq<int>), ((seq<int>), (seq<int>)), ((seq<int>), (seq<int>))), c: ((seq<int>), ((seq<int>), (seq<int>)), ((seq<int>), (seq<int>))))
+lemma MlJoinAssoc(a: (seq<int>, (seq<int>, seq<int>), (seq<int>, seq<int>)), b: (seq<int>, (seq<int>, seq<int>), (seq<int>, seq<int>)), c: (seq<int>, (seq<int>, seq<int>), (seq<int>, seq<int>)))
     decreases |a.0|, |a.1.0|, |a.1.1|, |a.2.0|, |a.2.1|, |b.0|, |b.1.0|, |b.1.1|, |b.2.0|, |b.2.1|, |c.0|, |c.1.0|, |c.1.1|, |c.2.0|, |c.2.1|
     requires |a.0| == |a.1.0| == |a.1.1| == |a.2.0| == |a.2.1| == |b.0| == |b.1.0| == |b.1.1| == |b.2.0| == |b.2.1| == |c.0| == |c.1.0| == |c.1.1| == |c.2.0| == |c.2.1|  && a.1.1 == a.2.1 && b.1.1 == b.2.1 && c.1.1 == c.2.1
     ensures MlJoin(MlJoin(a, b), c) == MlJoin(a, MlJoin(b, c))
 {
-    if |a.0| == 0 {}
-    else if |a.0| == 1 {}
+    var n := |a.0|;
+    if n == 0 {}
+    else if n == 1 {}
     else
     {
-        var a0' := a.0[..|a.0|-1];
-        var a10' := a.1.0[..|a.1.0|-1];
-        var a11' := a.1.1[..|a.1.1|-1];
-        var a20' := a.2.0[..|a.2.0|-1];
-        var a21' := a.2.1[..|a.2.1|-1];
-        var b0' := b.0[..|b.0|-1];
-        var b10' := b.1.0[..|b.1.0|-1];
-        var b11' := b.1.1[..|b.1.1|-1];
-        var b20' := b.2.0[..|b.2.0|-1];
-        var b21' := b.2.1[..|b.2.1|-1];
-        var c0' := c.0[..|c.0|-1];
-        var c10' := c.1.0[..|c.1.0|-1];
-        var c11' := c.1.1[..|c.1.1|-1];
-        var c20' := c.2.0[..|c.2.0|-1];
-        var c21' := c.2.1[..|c.2.1|-1];
+        var a0' := a.0[..n-1];
+        var a10' := a.1.0[..n-1];
+        var a11' := a.1.1[..n-1];
+        var a20' := a.2.0[..n-1];
+        var a21' := a.2.1[..n-1];
+        var b0' := b.0[..n-1];
+        var b10' := b.1.0[..n-1];
+        var b11' := b.1.1[..n-1];
+        var b20' := b.2.0[..n-1];
+        var b21' := b.2.1[..n-1];
+        var c0' := c.0[..n-1];
+        var c10' := c.1.0[..n-1];
+        var c11' := c.1.1[..n-1];
+        var c20' := c.2.0[..n-1];
+        var c21' := c.2.1[..n-1];
         MlJoinAssoc(((a0', (a10', a11'), (a20', a21'))), ((b0', (b10', b11'), (b20', b21'))), ((c0', (c10', c11'), (c20', c21'))));
 
-        var a0f := [a.0[|a.0|-1]];
-        var a10f := [a.1.0[|a.1.0|-1]];
-        var a11f := [a.1.1[|a.1.1|-1]];
-        var a20f := [a.2.0[|a.2.0|-1]];
-        var a21f := [a.2.1[|a.2.1|-1]];
-        var b0f := [b.0[|b.0|-1]];
-        var b10f := [b.1.0[|b.1.0|-1]];
-        var b11f := [b.1.1[|b.1.1|-1]];
-        var b20f := [b.2.0[|b.2.0|-1]];
-        var b21f := [b.2.1[|b.2.1|-1]];
-        var c0f := [c.0[|c.0|-1]];
-        var c10f := [c.1.0[|c.1.0|-1]];
-        var c11f := [c.1.1[|c.1.1|-1]];
-        var c20f := [c.2.0[|c.2.0|-1]];
-        var c21f := [c.2.1[|c.2.1|-1]];
+        var a0f := [a.0[n-1]];
+        var a10f := [a.1.0[n-1]];
+        var a11f := [a.1.1[n-1]];
+        var a20f := [a.2.0[n-1]];
+        var a21f := [a.2.1[n-1]];
+        var b0f := [b.0[n-1]];
+        var b10f := [b.1.0[n-1]];
+        var b11f := [b.1.1[n-1]];
+        var b20f := [b.2.0[n-1]];
+        var b21f := [b.2.1[n-1]];
+        var c0f := [c.0[n-1]];
+        var c10f := [c.1.0[n-1]];
+        var c11f := [c.1.1[n-1]];
+        var c20f := [c.2.0[n-1]];
+        var c21f := [c.2.1[n-1]];
         MlJoinAssoc(((a0f, (a10f, a11f), (a20f, a21f))), ((b0f, (b10f, b11f), (b20f, b21f))), ((c0f, (c10f, c11f), (c20f, c21f))));
     }
 }
