examples/mtlr_example/output.dfy
@@ -1,201 +1,206 @@
-function recSumS(s: seq2D): (seq<int>)
+function recSumS(s: seq2D): seq<int>
     ensures |recSumS(s)| == width(s)
 {
-    var recSumSRes := (if s == [] then [] else if |s| == 1 then preSum(s[0]) else vAdd(recSumS(s[..|s|-1]), preSum(s[|s|-1])));
+    var recSumSRes := if s == [] then [] else if |s| == 1 then preSum(s[0]) else vAdd(recSumS(s[..|s|-1]), preSum(s[|s|-1]));
     (recSumSRes)
 }
 
-function Mrr(s: seq2D): ((int), (seq<int>))
+function Mrr(s: seq2D): (int, seq<int>)
 {
-    var MrrRes := (if s == [] then 0 else if |s| == 1 then vMax(zeroSeq(|s[|s|-1]|), preSum(s[|s|-1])) else vMax(recSumS(s[..|s|-1]), preSum(s[|s|-1])));
+    var MrrRes := if s == [] then 0 else if |s| == 1 then vMax(zeroSeq(|s[|s|-1]|), preSum(s[|s|-1])) else vMax(recSumS(s[..|s|-1]), preSum(s[|s|-1]));
     var recSumSRes := recSumS(s);
     (MrrRes, recSumSRes)
 }
 
-function Mcr(s: seq2D): ((seq<int>), (seq<int>))
+function Mcr(s: seq2D): (seq<int>, seq<int>)
     ensures |Mcr(s).0| == width(s)
 {
-    var McrRes := (if s == [] then []  else if |s| == 1 then preSum(s[0]) else pMax(recSumS(s), Mcr(s[..|s|-1]).0));
+    var McrRes := if s == [] then []  else if |s| == 1 then preSum(s[0]) else pMax(recSumS(s), Mcr(s[..|s|-1]).0);
     var recSumSRes := recSumS(s);
     (McrRes, recSumSRes)
 }
 
-function Mtlr(s: seq2D): ((int), ((seq<int>), (seq<int>)))
+function Mtlr(s: seq2D): (int, (seq<int>, seq<int>))
 {
-    var MtlrRes := ((if s == [] then 0 else Max(Mtlr(s[..|s|-1]).0, Mrr(s).0)));
+    var MtlrRes := (if s == [] then 0 else Max(Mtlr(s[..|s|-1]).0, Mrr(s).0));
     var McrRes := Mcr(s);
     (MtlrRes, McrRes)
 }
 
-function Mblr(s: seq2D): ((seq<int>), (seq<int>))
+function Mblr(s: seq2D): (seq<int>, seq<int>)
     decreases |s|
 {
-    var MblrRes := (if s == [] then zeroSeq(width(s))
+    var MblrRes := if s == [] then zeroSeq(width(s))
                     else if |s| == 1 then pMax(zeroSeq(|s[|s|-1]|), preSum(s[|s|-1]))
                     else pMax(vAdd(Mblr(s[..|s|-1]).0, preSum(s[|s|-1])),
-                         Mblr([s[|s|-1]]).0));
+                         Mblr([s[|s|-1]]).0);
     var recSumSRes := recSumS(s);
     (MblrRes, recSumSRes)
 }
 
-function recSumSJoin(a: (seq<int>), b: (seq<int>)): (seq<int>)
+function recSumSJoin(a: seq<int>, b: seq<int>): seq<int>
     requires |a| == |b|
 {
-    var recSumSRes := (vAdd(a, b));
+    var recSumSRes := vAdd(a, b);
     (recSumSRes)
 }
 
-function MrrJoin(a: ((int), (seq<int>)), b: ((int), (seq<int>))): ((int), (seq<int>))
+function MrrJoin(a: (int, seq<int>), b: (int, seq<int>)): (int, seq<int>)
     requires |a.1| == |b.1|
 {
-    var MrrRes := (vMax(a.1, b.1));
+    var MrrRes := vMax(a.1, b.1);
     var recSumSRes := recSumSJoin(a.1, b.1);
     (MrrRes, recSumSRes)
 }
 
-function McrJoin(a: ((seq<int>), (seq<int>)), b: ((seq<int>), (seq<int>))): ((seq<int>), (seq<int>))
+function McrJoin(a: (seq<int>, seq<int>), b: (seq<int>, seq<int>)): (seq<int>, seq<int>)
     requires |a.0| == |a.1| == |b.0| == |b.1|
 {
-    var McrRes := (pMax(vAdd(a.1, b.0), a.0));
+    var McrRes := pMax(vAdd(a.1, b.0), a.0);
     var recSumSRes := recSumSJoin(a.1, b.1);
     (McrRes, recSumSRes)
 }
 
-function MtlrJoin(a: ((int), ((seq<int>), (seq<int>))), b: ((int), ((seq<int>), (seq<int>)))): ((int), ((seq<int>), (seq<int>)))
+function MtlrJoin(a: (int, (seq<int>, seq<int>)), b: (int, (seq<int>, seq<int>))): (int, (seq<int>, seq<int>))
     requires |a.1.0| == |a.1.1| == |b.1.0| == |b.1.1|
 {
-    var MtlrRes := (Max(a.0, vMax(a.1.1, b.1.0)));
+    var MtlrRes := Max(a.0, vMax(a.1.1, b.1.0));
     var McrRes := McrJoin(a.1, b.1);
     (MtlrRes, McrRes)
 }
 
-function MblrJoin(a: ((seq<int>), (seq<int>)), b: ((seq<int>), (seq<int>))): ((seq<int>), (seq<int>))
+function MblrJoin(a: (seq<int>, seq<int>), b: (seq<int>, seq<int>)): (seq<int>, seq<int>)
     requires |a.0| == |a.1| == |b.0| == |b.1|
 {
-    var MblrRes := (pMax(vAdd(a.0, b.1), b.0));
+    var MblrRes := pMax(vAdd(a.0, b.1), b.0);
     var recSumSRes := recSumSJoin(a.1, b.1);
     (MblrRes, recSumSRes)
 }
 
-lemma recSumSJoinAssoc(a: (seq<int>), b: (seq<int>), c: (seq<int>))
+lemma recSumSJoinAssoc(a: seq<int>, b: seq<int>, c: seq<int>)
     decreases |a|, |b|, |c|
     requires |a| == |b| == |c| 
     ensures recSumSJoin(recSumSJoin(a, b), c) == recSumSJoin(a, recSumSJoin(b, c))
 {
-    if |a| == 0 {}
-    else if |a| == 1 {}
+    var n := |a|;
+    if n == 0 {}
+    else if n == 1 {}
     else
     {
-        var a' := a[..|a|-1];
-        var b' := b[..|b|-1];
-        var c' := c[..|c|-1];
+        var a' := a[..n-1];
+        var b' := b[..n-1];
+        var c' := c[..n-1];
         recSumSJoinAssoc((a'), (b'), (c'));
 
-        var af := [a[|a|-1]];
-        var bf := [b[|b|-1]];
-        var cf := [c[|c|-1]];
+        var af := [a[n-1]];
+        var bf := [b[n-1]];
+        var cf := [c[n-1]];
         recSumSJoinAssoc((af), (bf), (cf));
     }
 }
 
-lemma MrrJoinAssoc(a: ((int), (seq<int>)), b: ((int), (seq<int>)), c: ((int), (seq<int>)))
+lemma MrrJoinAssoc(a: (int, seq<int>), b: (int, seq<int>), c: (int, seq<int>))
     decreases |a.1|, |b.1|, |c.1|
     requires |a.1| == |b.1| == |c.1| 
     ensures MrrJoin(MrrJoin(a, b), c) == MrrJoin(a, MrrJoin(b, c))
 {
-    if |a.1| == 0 {}
-    else if |a.1| == 1 {}
+    var n := |a.1|;
+    if n == 0 {}
+    else if n == 1 {}
     else
     {
-        var a1' := a.1[..|a.1|-1];
-        var b1' := b.1[..|b.1|-1];
-        var c1' := c.1[..|c.1|-1];
+        var a1' := a.1[..n-1];
+        var b1' := b.1[..n-1];
+        var c1' := c.1[..n-1];
         MrrJoinAssoc((((a.0), a1')), (((b.0), b1')), (((c.0), c1')));
 
-        var a1f := [a.1[|a.1|-1]];
-        var b1f := [b.1[|b.1|-1]];
-        var c1f := [c.1[|c.1|-1]];
+        var a1f := [a.1[n-1]];
+        var b1f := [b.1[n-1]];
+        var c1f := [c.1[n-1]];
         MrrJoinAssoc((((a.0), a1f)), (((b.0), b1f)), (((c.0), c1f)));
     }
 }
 
-lemma McrJoinAssoc(a: ((seq<int>), (seq<int>)), b: ((seq<int>), (seq<int>)), c: ((seq<int>), (seq<int>)))
+lemma McrJoinAssoc(a: (seq<int>, seq<int>), b: (seq<int>, seq<int>), c: (seq<int>, seq<int>))
     decreases |a.0|, |a.1|, |b.0|, |b.1|, |c.0|, |c.1|
     requires |a.0| == |a.1| == |b.0| == |b.1| == |c.0| == |c.1| 
     ensures McrJoin(McrJoin(a, b), c) == McrJoin(a, McrJoin(b, c))
 {
-    if |a.0| == 0 {}
-    else if |a.0| == 1 {}
+    var n := |a.0|;
+    if n == 0 {}
+    else if n == 1 {}
     else
     {
-        var a0' := a.0[..|a.0|-1];
-        var a1' := a.1[..|a.1|-1];
-        var b0' := b.0[..|b.0|-1];
-        var b1' := b.1[..|b.1|-1];
-        var c0' := c.0[..|c.0|-1];
-        var c1' := c.1[..|c.1|-1];
+        var a0' := a.0[..n-1];
+        var a1' := a.1[..n-1];
+        var b0' := b.0[..n-1];
+        var b1' := b.1[..n-1];
+        var c0' := c.0[..n-1];
+        var c1' := c.1[..n-1];
         McrJoinAssoc(((a0', a1')), ((b0', b1')), ((c0', c1')));
 
-        var a0f := [a.0[|a.0|-1]];
-        var a1f := [a.1[|a.1|-1]];
-        var b0f := [b.0[|b.0|-1]];
-        var b1f := [b.1[|b.1|-1]];
-        var c0f := [c.0[|c.0|-1]];
-        var c1f := [c.1[|c.1|-1]];
+        var a0f := [a.0[n-1]];
+        var a1f := [a.1[n-1]];
+        var b0f := [b.0[n-1]];
+        var b1f := [b.1[n-1]];
+        var c0f := [c.0[n-1]];
+        var c1f := [c.1[n-1]];
         McrJoinAssoc(((a0f, a1f)), ((b0f, b1f)), ((c0f, c1f)));
     }
 }
 
-lemma MtlrJoinAssoc(a: ((int), ((seq<int>), (seq<int>))), b: ((int), ((seq<int>), (seq<int>))), c: ((int), ((seq<int>), (seq<int>))))
+lemma MtlrJoinAssoc(a: (int, (seq<int>, seq<int>)), b: (int, (seq<int>, seq<int>)), c: (int, (seq<int>, seq<int>)))
     decreases |a.1.0|, |a.1.1|, |b.1.0|, |b.1.1|, |c.1.0|, |c.1.1|
     requires |a.1.0| == |a.1.1| == |b.1.0| == |b.1.1| == |c.1.0| == |c.1.1| 
     ensures MtlrJoin(MtlrJoin(a, b), c) == MtlrJoin(a, MtlrJoin(b, c))
 {
-    if |a.1.0| == 0 {}
-    else if |a.1.0| == 1 {}
+    var n := |a.1.0|;
+    if n == 0 {}
+    else if n == 1 {}
     else
     {
-        var a10' := a.1.0[..|a.1.0|-1];
-        var a11' := a.1.1[..|a.1.1|-1];
-        var b10' := b.1.0[..|b.1.0|-1];
-        var b11' := b.1.1[..|b.1.1|-1];
-        var c10' := c.1.0[..|c.1.0|-1];
-        var c11' := c.1.1[..|c.1.1|-1];
+        var a10' := a.1.0[..n-1];
+        var a11' := a.1.1[..n-1];
+        var b10' := b.1.0[..n-1];
+        var b11' := b.1.1[..n-1];
+        var c10' := c.1.0[..n-1];
+        var c11' := c.1.1[..n-1];
         MtlrJoinAssoc((((a.0), (a10', a11'))), (((b.0), (b10', b11'))), (((c.0), (c10', c11'))));
 
-        var a10f := [a.1.0[|a.1.0|-1]];
-        var a11f := [a.1.1[|a.1.1|-1]];
-        var b10f := [b.1.0[|b.1.0|-1]];
-        var b11f := [b.1.1[|b.1.1|-1]];
-        var c10f := [c.1.0[|c.1.0|-1]];
-        var c11f := [c.1.1[|c.1.1|-1]];
+        var a10f := [a.1.0[n-1]];
+        var a11f := [a.1.1[n-1]];
+        var b10f := [b.1.0[n-1]];
+        var b11f := [b.1.1[n-1]];
+        var c10f := [c.1.0[n-1]];
+        var c11f := [c.1.1[n-1]];
         MtlrJoinAssoc((((a.0), (a10f, a11f))), (((b.0), (b10f, b11f))), (((c.0), (c10f, c11f))));
     }
 }
 
-lemma MblrJoinAssoc(a: ((seq<int>), (seq<int>)), b: ((seq<int>), (seq<int>)), c: ((seq<int>), (seq<int>)))
+lemma MblrJoinAssoc(a: (seq<int>, seq<int>), b: (seq<int>, seq<int>), c: (seq<int>, seq<int>))
     decreases |a.0|, |a.1|, |b.0|, |b.1|, |c.0|, |c.1|
     requires |a.0| == |a.1| == |b.0| == |b.1| == |c.0| == |c.1| 
     ensures MblrJoin(MblrJoin(a, b), c) == MblrJoin(a, MblrJoin(b, c))
 {
-    if |a.0| == 0 {}
-    else if |a.0| == 1 {}
+    var n := |a.0|;
+    if n == 0 {}
+    else if n == 1 {}
     else
     {
-        var a0' := a.0[..|a.0|-1];
-        var a1' := a.1[..|a.1|-1];
-        var b0' := b.0[..|b.0|-1];
-        var b1' := b.1[..|b.1|-1];
-        var c0' := c.0[..|c.0|-1];
-        var c1' := c.1[..|c.1|-1];
+        var a0' := a.0[..n-1];
+        var a1' := a.1[..n-1];
+        var b0' := b.0[..n-1];
+        var b1' := b.1[..n-1];
+        var c0' := c.0[..n-1];
+        var c1' := c.1[..n-1];
         MblrJoinAssoc(((a0', a1')), ((b0', b1')), ((c0', c1')));
 
-        var a0f := [a.0[|a.0|-1]];
-        var a1f := [a.1[|a.1|-1]];
-        var b0f := [b.0[|b.0|-1]];
-        var b1f := [b.1[|b.1|-1]];
-        var c0f := [c.0[|c.0|-1]];
-        var c1f := [c.1[|c.1|-1]];
+        var a0f := [a.0[n-1]];
+        var a1f := [a.1[n-1]];
+        var b0f := [b.0[n-1]];
+        var b1f := [b.1[n-1]];
+        var c0f := [c.0[n-1]];
+        var c1f := [c.1[n-1]];
         MblrJoinAssoc(((a0f, a1f)), ((b0f, b1f)), ((c0f, c1f)));
     }
 }
